\documentclass{ctexart}
  \usepackage{amsmath}
  \usepackage{amssymb}
  \usepackage{graphicx}
  \usepackage{float}
  \usepackage{setspace}
\topmargin=-1.2cm \oddsidemargin=0.1cm \evensidemargin=0.1cm
\textwidth=16 true cm \textheight=23 true cm

\font\euler=EUSM10 \font\eulers=EUSM7

\begin{document}
\title{数学双学位：统计学 \\第11次作业}
\author{{\normalsize 盛浩, 学号:1000017438, \LaTeX}}
\date{\today}

\maketitle

\def \Pr{{\rm Pr}}

\baselineskip 0.6cm
{\bf 习题九}
\begin{description}
    \item[8.]{\bf 解：}\\
        \begin{description}
          \item[i.]
            \begin{align}
              Y&=\text{Xb}+e\\
              \intertext{其中,}
              X&=\left(\begin{array}{ccc} 1 & 1 & 0 \\ 1 & 1 & 1 \\ 1 & 0 & 1 \\ 1 & 0 & 0\end{array}\right),b=\left(\begin{array}{c} \theta _1 \\ \theta _2 \\ \theta _3\end{array}\right),e\sim N\left(0,\sigma ^2I_n\right)
            \end{align}
          \item[ii.]
            记,
            \begin{align}
              \hat{b}&=\left(X^TX\right)^{-1}X^TY\\
              (Y-\text{Xb})^T(Y-\text{Xb})&=\left(\left(Y-X\hat{b}\right)+X\left(\hat{b}-b\right)\right)^T\left(\left(Y-X\hat{b}\right)+X\left(\hat{b}-b\right)\right)\\
              \intertext{由于,}
              \left(X\left(\hat{b}-b\right)\right)^T(Y-\text{Xb})&=\left(\hat{b}-b\right)^T\left(X^TY-X^TX\left(X^TX\right)^{-1}X^TY\right)=0\\
              (Y-\text{Xb})^T(Y-\text{Xb})&=\left(Y-X\hat{b}\right)^T\left(Y-X\hat{b}\right)+X\left(\hat{b}-b\right)^TX\left(\hat{b}-b\right)
            \end{align}
            由$b$的任意性, $\hat{b}$为$b=\left(\begin{array}{c} \theta _1 \\ \theta _2 \\ \theta _3\end{array}\right)$最小二乘估计.
.          \item[iii.]
            \begin{align}
              \hat{\sigma }^2=\frac{\left(Y-X\hat{b}\right)^T\left(Y-X\hat{b}\right)}{n-p}=\frac{\left(y_1-y_2+y_3-y_4\right){}^2}{4}
            \end{align}
        \end{description}
\end{description}
\newpage
{\bf 补充题}
\begin{description}
    \item[1.]{\bf 解：}\\
        \begin{align}
          \left(\left\|X_1+X_2\right\|\right){}^2&=\left(X_1+X_2\right){}^T\left(X_1+X_2\right)\\
          &=X_1{}^TX_1+X_2{}^TX_2+2\left(X_1\right){}^TX_2\\
          &=\left(\left\|X_1\right\|\right){}^2+\left(\left\|X_2\right\|\right){}^2
        \end{align}
    \item[2.]{\bf 解：}\\
        \begin{align}
          &\left(\tilde{Y}-\tilde{X}\hat{b}\right)+\tilde{X}\left(\hat{b}-b\right)+1\left(\overset{-}{Y}-\overset{-}{X}b-b_0\right)\\
          &=\left(\tilde{Y}+1\overset{-}{Y}\right)-\left(\tilde{X}+1\overset{-}{X}\right)b-1b_0\\
          &=Y-1b_0-\text{Xb}
        \end{align}
\end{description}
\end{document}
